Lean4Lean/Std/Basic.lean
@@ -1,6 +1,7 @@
 import Batteries.CodeAction
 import Batteries.Data.Array.Lemmas
 import Batteries.Data.HashMap.Basic
+import Batteries.Tactic.SeqFocus
 
 attribute [simp] Option.bind_eq_some List.filterMap_cons
 
@@ -101,26 +102,13 @@ theorem List.idxOf_eq_length_iff [BEq α] [LawfulBEq α]
   induction l with
   | nil => exact iff_of_true rfl not_mem_nil
   | cons b l ih =>
-    simp only [length, mem_cons, idxOf_cons, eq_comm]
+    simp only [length, mem_cons, idxOf_cons]
     rw [cond_eq_if]
     split <;> rename_i h <;> simp at h
     · exact iff_of_false (by rintro ⟨⟩) fun H => H <| Or.inl h.symm
     · simp only [Ne.symm h, false_or]
       rw [← ih]
       exact Nat.succ_inj
-
-theorem List.idxOf_le_length [BEq α] [LawfulBEq α]
-    {a : α} {l : List α} : idxOf a l ≤ length l := by
-  induction l with | nil => exact Nat.le_refl _ | cons b l ih => ?_
-  simp only [length, idxOf_cons, cond_eq_if, beq_iff_eq]
-  by_cases h : b == a
-  · rw [if_pos h]; exact Nat.zero_le _
-  · rw [if_neg h]; exact Nat.succ_le_succ ih
-
-theorem List.idxOf_lt_length_iff [BEq α] [LawfulBEq α]
-    {a} {l : List α} : idxOf a l < length l ↔ a ∈ l :=
-  ⟨fun h => Decidable.byContradiction fun al => Nat.ne_of_lt h <| idxOf_eq_length_iff.2 al,
-   fun al => (Nat.lt_of_le_of_ne idxOf_le_length) fun h => idxOf_eq_length_iff.1 h al⟩
 
 instance [BEq α] [LawfulBEq α] : PartialEquivBEq α where
   symm h := by simp at *; exact h.symm
